filling in SeparationLogic interface
We don't have the logic-vs-pred distinction anymore, so I tried deduplicating definitions wherever possible.

veric/SeparationLogic.v
@@ -14,6 +14,8 @@ Require Export VST.veric.tycontext.
 Require Export VST.veric.change_compspecs.
 Require Export VST.veric.mpred.
 Require Export VST.veric.expr.
+Require Export VST.veric.expr2.
+Require Export VST.veric.expr_lemmas.
 Require Export VST.veric.Clight_lemmas.
 Require Export VST.veric.composite_compute.
 Require Export VST.veric.align_mem.
@@ -21,9 +23,18 @@ Require Export VST.veric.shares.
 Require Export VST.veric.seplog.
 Require Export VST.veric.Clight_seplog.
 Require Export VST.veric.Clight_assert_lemmas.
+Require Export VST.veric.extend_tc.
 Require Import VST.msl.Coqlib2.
 Require Import VST.veric.juicy_extspec.
+Require Import VST.veric.mapsto_memory_block.
 Require Import VST.veric.valid_pointer.
+Require Export VST.veric.external_state.
+Require Export VST.veric.Clight_initial_world.
+Require Export VST.veric.initialize.
+Require Export VST.veric.semax.
+Require Export VST.veric.juicy_mem_lemmas.
+Require Export VST.veric.semax_straight.
+Require Export VST.veric.semax_call.
 Require Export VST.veric.semax_prog.
 Require Export VST.veric.semax_ext.
 Import LiftNotation.
@@ -34,11 +45,15 @@ Import Ctypes Clight expr.
 #[export] Existing Instance EqDec_memval.
 #[export] Existing Instance EqDec_quantity.
 
-Definition local:  (environ -> Prop) -> environ->mpred :=  lift1 prop.
-
 Global Opaque mpred.
 
 #[export] Hint Resolve any_environ : typeclass_instances.
+
+Section mpred.
+
+Context `{!heapGS Σ}.
+
+Definition local:  (environ -> Prop) -> assert := fun l => assert_of (lift1 bi_pure l).
 
 (* Somehow, this fixes a universe collapse issue that will occur if fool is not defined.
 Definition fool := @map _ Type (fun it : ident * type => mpred).*)
@@ -63,18 +78,16 @@ Definition ext_link_prog (p: program) (s: String.string) : ident :=
 
 Definition globals := ident -> val.
 
+
 (*We're exporting the step-indexed version so that semax_fun_id doesn't syntactically change*)
-Definition func_ptr (f: funspec) (v: val): mpred := seplog.func_ptr_si f v.
+Definition func_ptr ge E id (f: funspec) (v: val): mpred := seplog.func_ptr_si ge E id f v.
 
 (*veric.seplog has a lemma that weakens the hypothesis here to funspec_sub_si*)
-Lemma func_ptr_mono fs gs v (H:funspec_sub fs gs): func_ptr fs v |-- func_ptr gs v.
-Proof. constructor; apply funspec_sub_implies_func_prt_si_mono.
-       now rewrite <- funspec_sub_iff.
-Qed.
+Lemma func_ptr_mono ge E id fs gs v (H:funspec_sub E fs gs): func_ptr ge E id fs v ⊢ func_ptr ge E id gs v.
+Proof. apply funspec_sub_implies_func_prt_si_mono; done. Qed.
 
-Lemma func_ptr_isptr: forall spec f, func_ptr spec f |-- !! isptr f.
-Proof. constructor; apply seplog.func_ptr_si_isptr.
-Qed.
+Lemma func_ptr_isptr: forall ge E id spec f, func_ptr ge E id spec f ⊢ ⌜isptr f⌝.
+Proof. apply seplog.func_ptr_si_isptr. Qed.
 
 Definition type_of_funsig (fsig: funsig) :=
    Tfunction (type_of_params (fst fsig)) (snd fsig) cc_default.
@@ -88,27 +101,20 @@ Fixpoint arglist (n: positive) (tl: typelist) : list (ident*type) :=
   | Tcons t tl' => (n,t):: arglist (n+1)%positive tl'
  end.
 
-Definition  funspecs_norepeat (fs : funspecs) := list_norepet (map fst fs).
-
 (* Misc lemmas *)
 Lemma typecheck_lvalue_sound {CS: compspecs} :
   forall Delta rho e,
     typecheck_environ Delta rho ->
-    tc_lvalue Delta e rho |-- !! is_pointer_or_null (eval_lvalue e rho).
+    tc_lvalue Delta e rho ⊢ ⌜is_pointer_or_null (eval_lvalue e rho)⌝.
 Proof.
-constructor; intros.
-intros ? ?.
 eapply expr_lemmas4.typecheck_lvalue_sound; eauto.
 Qed.
 
 Lemma typecheck_expr_sound {CS: compspecs} :
   forall Delta rho e,
     typecheck_environ Delta rho ->
-    tc_expr Delta e rho |-- !! tc_val (typeof e) (eval_expr e rho).
+    tc_expr Delta e rho ⊢ ⌜tc_val (typeof e) (eval_expr e rho)⌝.
 Proof.
-constructor; intros.
-intros ? ?.
-simpl.
 eapply expr_lemmas4.typecheck_expr_sound; eauto.
 Qed.
 
@@ -116,72 +122,53 @@ Qed.
 
 Lemma tc_expr_cspecs_sub: forall {CS CS'} (CSUB: cspecs_sub  CS CS') Delta e rho,
   tc_environ Delta rho ->
-  @tc_expr CS Delta e rho |-- @tc_expr CS' Delta e rho.
-Proof. intros. destruct CSUB as [CSUB _]. rewrite tc_expr_eq. constructor; intros w W. apply (extend_tc.tc_expr_cenv_sub CSUB e rho Delta). trivial. Qed.
-
-Lemma tc_expropt_char {CS} Delta e t: @tc_expropt CS Delta e t =
-                                      match e with None => `!!(t=Tvoid)
-                                              | Some e' => @tc_expr CS Delta (Ecast e' t)
-                                      end.
-Proof. reflexivity. Qed.
-
-Lemma tc_expropt_cenv_sub {CS CS'} (CSUB: cspecs_sub CS CS') Delta rho (D:typecheck_environ Delta rho) ret t:
-  @tc_expropt CS Delta ret t rho |-- @tc_expropt CS' Delta ret t rho.
-Proof.
-  destruct ret; simpl. 2: constructor; apply  predicates_hered.derives_refl.
-  apply (tc_expr_cspecs_sub CSUB Delta (Ecast e t) rho D). 
-Qed.
+  tc_expr(CS := CS) Delta e rho ⊢ tc_expr (CS := CS') Delta e rho.
+Proof. intros. destruct CSUB as [CSUB _]. apply (extend_tc.tc_expr_cenv_sub CSUB e rho Delta). Qed.
 
 Lemma tc_lvalue_cspecs_sub: forall {CS CS'} (CSUB: cspecs_sub  CS CS') Delta e rho,
   tc_environ Delta rho ->
-  @tc_lvalue CS Delta e rho |-- @tc_lvalue CS' Delta e rho.
-Proof. intros; simpl. destruct CSUB as [CSUB _]. constructor; red; intros. apply (extend_tc.tc_lvalue_cenv_sub CSUB e rho Delta). apply H0. Qed.
+  tc_lvalue (CS := CS) Delta e rho ⊢ tc_lvalue (CS := CS') Delta e rho.
+Proof. intros; simpl. destruct CSUB as [CSUB _]. apply (extend_tc.tc_lvalue_cenv_sub CSUB e rho Delta). Qed.
 
 Lemma tc_exprlist_cspecs_sub {CS CS'} (CSUB: cspecs_sub  CS CS') Delta rho: forall types e,
   tc_environ Delta rho ->
-  @tc_exprlist CS Delta types e rho |-- @tc_exprlist CS' Delta types e rho.
-Proof. intros. destruct CSUB as [CSUB _]. constructor; intros w W. apply (extend_tc.tc_exprlist_cenv_sub CSUB Delta rho w types e W). Qed.
+  tc_exprlist (CS := CS) Delta types e rho ⊢ tc_exprlist (CS := CS') Delta types e rho.
+Proof. intros. destruct CSUB as [CSUB _]. apply (extend_tc.tc_exprlist_cenv_sub CSUB Delta rho). Qed.
 
 Lemma eval_exprlist_cspecs_sub {CS CS'} (CSUB: cspecs_sub  CS CS') Delta rho (TCD: tc_environ Delta rho):
   forall types e,
-  @tc_exprlist CS Delta types e rho |-- !! (@eval_exprlist CS types e rho = @eval_exprlist CS' types e rho).
-Proof. intros. destruct CSUB as [CSUB _]. constructor; intros w W. eapply (expr_lemmas.typecheck_exprlist_sound_cenv_sub CSUB); eassumption. Qed.
+  tc_exprlist (CS := CS) Delta types e rho ⊢ ⌜@eval_exprlist CS types e rho = @eval_exprlist CS' types e rho⌝.
+Proof. intros. destruct CSUB as [CSUB _]. eapply (expr_lemmas.typecheck_exprlist_sound_cenv_sub CSUB); eassumption. Qed.
 
 Lemma denote_tc_assert_tc_bool_cs_invariant {CS CS'} b E:
-  @denote_tc_assert CS (tc_bool b E) = @denote_tc_assert CS' (tc_bool b E).
+  denote_tc_assert (CS := CS) (tc_bool b E) = denote_tc_assert (CS := CS') (tc_bool b E).
 Proof. unfold tc_bool. destruct b; reflexivity. Qed.
 
 Lemma tc_temp_id_cspecs_sub {CS CS'} (CSUB: cspecs_sub  CS CS') Delta rho e i:
-  tc_environ Delta rho -> @tc_temp_id i (typeof e) CS Delta e rho |-- @tc_temp_id i (typeof e) CS' Delta e rho.
+  tc_environ Delta rho -> tc_temp_id i (typeof e) (CS := CS) Delta e rho ⊢ tc_temp_id i (typeof e) (CS := CS') Delta e rho.
 Proof.
-  intros. constructor; unfold tc_temp_id, typecheck_temp_id; intros w W.
-  destruct ((temp_types Delta)! i); [| apply W].
-  rewrite denote_tc_assert_andp in W.
-  rewrite denote_tc_assert_andp; destruct W as [W1 W2];  split.
-+ rewrite (@denote_tc_assert_tc_bool_cs_invariant CS' CS). exact W1. 
-+ apply expr2.tc_bool_e in W1. eapply expr2.neutral_isCastResultType.
-  exact W1.
-Qed. 
+  intros. unfold tc_temp_id, typecheck_temp_id; simpl.
+  destruct ((temp_types Delta) !! i); last done.
+  rewrite !denote_tc_assert_andp.
+  iIntros "H"; iSplit.
+  + iDestruct "H" as "[H _]"; rewrite (@denote_tc_assert_tc_bool_cs_invariant CS' CS) //.
+  + rewrite tc_bool_e; iDestruct "H" as (?) "?".
+    iApply expr2.neutral_isCastResultType.
+Qed.
 
-(*Proof exists in semax_call under name RA_return_castexpropt_cenv_sub -- repeat here for the exposed def of castexprof?*)
 Lemma castexpropt_cenv_sub {CS CS'} (CSUB: cspecs_sub CS CS') Delta rho (D:typecheck_environ Delta rho) ret t:
-  @tc_expropt CS Delta ret t rho |-- !!(@cast_expropt CS ret t rho = @cast_expropt CS' ret t rho).
+  tc_expropt (CS := CS) Delta ret t rho ⊢ ⌜@cast_expropt CS ret t rho = @cast_expropt CS' ret t rho⌝.
 Proof.
-  constructor; intros w W. destruct CSUB as [CSUB _]. rewrite tc_expropt_char in W. destruct ret; [ | reflexivity].
-  specialize (expr_lemmas.typecheck_expr_sound_cenv_sub CSUB Delta rho D w (Ecast e t) W); clear W; intros H.
-  hnf. unfold cast_expropt. simpl; simpl in H. 
-  unfold force_val1, force_val, sem_cast, liftx, lift; simpl.
-  unfold force_val1, force_val, sem_cast, liftx, lift in H; simpl in H. rewrite H; trivial.
+  destruct CSUB; apply RA_return_castexpropt_cenv_sub; done.
 Qed.
 
 Lemma RA_return_cast_expropt_cspecs_sub: forall {CS CS'} (CSUB: cspecs_sub  CS CS') Delta e t R rho,
   tc_environ Delta rho ->
-  @tc_expropt CS Delta e t rho && RA_return R (@cast_expropt CS e t rho) (id rho)
-  |-- RA_return R (@cast_expropt CS' e t rho) (id rho).
+  tc_expropt (CS := CS) Delta e t rho ∧ RA_return R (@cast_expropt CS e t rho) (id rho)
+  ⊢ RA_return R (@cast_expropt CS' e t rho) (id rho).
 Proof.
-  intros. constructor; intros w [W1 W2].
-  pose proof (castexpropt_cenv_sub CSUB _ _ H e t) as H1. unseal_derives.
-  rewrite (H1 w W1) in W2. apply W2.
+  intros. rewrite castexpropt_cenv_sub //.
+  iIntros "(-> & $)".
 Qed.
 
 (********************************************* LENB: END OF ADDED LEMMAS********************)
@@ -208,54 +195,49 @@ with nocontinue_ls sl :=
  match sl with LSnil => true | LScons _ s sl' => if nocontinue s then nocontinue_ls sl' else false
  end.
 
-Definition withtype_empty (A: rmaps.TypeTree) : Prop :=
-  forall ts : list Type,
- functors.MixVariantFunctor._functor
-   (rmaps.dependent_type_functor_rec ts A)
-   (predicates_hered.pred compcert_rmaps.RML.R.rmap) -> False.
+End mpred.
 
 Module Type CLIGHT_SEPARATION_HOARE_LOGIC_DEF.
 
-Parameter semax: forall {CS: compspecs} {Espec: OracleKind},
-    tycontext -> (environ->mpred) -> statement -> ret_assert -> Prop.
+Parameter semax: forall {Σ : gFunctors} `{!heapGS Σ} {Espec : OracleKind}
+  `{!externalGS (OK_ty(Σ := Σ)) Σ} {C : compspecs},
+  coPset → tycontext → (environ → mpred) → statement → ret_assert → Prop.
 
-Parameter semax_func:
-    forall {Espec: OracleKind},
-    forall (V: varspecs) (G: funspecs) {C: compspecs} (ge: Genv.t fundef type) (fdecs: list (ident * fundef)) (G1: funspecs), Prop.
+Parameter semax_func: forall {Σ : gFunctors} `{!heapGS Σ} {Espec : OracleKind}
+  `{!externalGS (OK_ty(Σ := Σ)) Σ} (V : varspecs) (G : @funspecs Σ) {C : compspecs},
+  Genv.t fundef type → coPset → list (ident * fundef) → @funspecs Σ → Prop.
 
-Parameter semax_external: forall {Hspec: OracleKind} (ef: external_function) (A : rmaps.TypeTree)
-       (P: forall ts : list Type, functors.MixVariantFunctor._functor (rmaps.dependent_type_functor_rec ts (ArgsTT A)) mpred)
-       (Q: forall ts : list Type, functors.MixVariantFunctor._functor (rmaps.dependent_type_functor_rec ts (AssertTT A)) mpred), Prop.
+Parameter semax_external: forall {Σ : gFunctors} {heapGS0 : heapGS Σ} {Espec : OracleKind}
+  `{!externalGS (OK_ty(Σ := Σ)) Σ}, coPset → external_function →
+  ∀ A : Type, (A → argsEnviron → mpred) → (A → environ → mpred) → mpred.
 
 End CLIGHT_SEPARATION_HOARE_LOGIC_DEF.
 
 Module DerivedDefs (Def: CLIGHT_SEPARATION_HOARE_LOGIC_DEF).
 
-Local Open Scope pred.
-
-Definition semax_body
-   (V: varspecs) (G: funspecs) {C: compspecs} (f: function) (spec: ident * funspec): Prop :=
-match spec with (_, mk_funspec fsig cc A P Q _ _) =>
-  fst fsig = map snd (fst (fn_funsig f)) /\ 
+Definition semax_body `{!heapGS Σ} {Espec} `{!externalGS OK_ty Σ}
+   (V: varspecs) (G: funspecs) {C: compspecs} E (f: function) (spec: ident * funspec): Prop :=
+match spec with (_, mk_funspec fsig cc A P Q) =>
+  fst fsig = map snd (fst (fn_funsig f)) /\
   snd fsig = snd (fn_funsig f) /\
-forall Espec ts x,
-  @Def.semax C Espec (func_tycontext f V G nil)
-      (fun rho => close_precondition (map fst f.(fn_params)) (P ts x) rho * stackframe_of f rho)
+forall (x:A),
+  Def.semax E (func_tycontext f V G nil)
+      (fun rho => close_precondition (map fst f.(fn_params)) (P x) rho ∗ stackframe_of f rho)
        f.(fn_body)
-      (frame_ret_assert (function_body_ret_assert (fn_return f) (Q ts x)) (stackframe_of f))
+      (frame_ret_assert (function_body_ret_assert (fn_return f) (Q x)) (stackframe_of f))
 end.
 
-Definition semax_prog {Espec: OracleKind}{C: compspecs}
-       (prog: program) (z: OK_ty) (V: varspecs) (G: funspecs) : Prop :=
+Definition semax_prog `{!heapGS Σ} {Espec} `{!externalGS OK_ty Σ} {C: compspecs}
+       (prog: program) (ora: OK_ty) (V: varspecs) (G: funspecs) : Prop :=
 compute_list_norepet (prog_defs_names prog) = true  /\
 all_initializers_aligned prog /\
-PTree.elements cenv_cs = PTree.elements (prog_comp_env prog) /\
-  @Def.semax_func Espec V G C (Genv.globalenv prog)  (prog_funct prog) G /\
-  match_globvars (prog_vars prog) V = true /\
-  match initial_world.find_id prog.(prog_main) G with
-  | Some s => exists post,
-             s = main_spec_ext' prog z post
-  | None => False
+Maps.PTree.elements cenv_cs = Maps.PTree.elements (prog_comp_env prog) /\
+Def.semax_func V G (Genv.globalenv prog) ⊤ (prog_funct prog) G /\
+match_globvars (prog_vars prog) V = true /\
+match find_id prog.(prog_main) G with
+| Some s => exists post,
+      s = main_spec_ext' prog ora post
+| None => False
 end.
 
 End DerivedDefs.
@@ -271,18 +253,20 @@ Import CSHL_Defs.
 
 (***************** SEMAX_LEMMAS ****************)
 
+Section mpred.
+
+Context `{!heapGS Σ} {Espec: OracleKind} `{!externalGS (OK_ty(Σ := Σ)) Σ} {CS: compspecs}.
+
 Axiom semax_extract_exists:
-  forall {CS: compspecs} {Espec: OracleKind},
-  forall (A : Type) (P : A -> environ->mpred) c (Delta: tycontext) (R: ret_assert),
-  (forall x, @semax CS Espec Delta (P x) c R) ->
-   @semax CS Espec Delta (EX x:A, P x) c R.
+  forall E (A : Type) (P : A -> assert) c (Delta: tycontext) (R: ret_assert),
+  (forall x, semax E Delta (P x) c R) ->
+   semax E Delta (∃ x:A, P x) c R.
   
-Axiom semax_func_nil:   forall {Espec: OracleKind},
-        forall V G C ge, @semax_func Espec V G C ge nil nil.
+Axiom semax_func_nil:
+        forall V G E ge, semax_func V G E ge nil nil.
 
 Axiom semax_func_cons:
-  forall {Espec: OracleKind},
-     forall fs id f fsig cc A P Q NEP NEQ (V: varspecs) (G G': funspecs) {C: compspecs} ge b,
+     forall fs id f fsig cc A P Q (V: varspecs) (G G': funspecs) ge E b,
   andb (id_in_list id (map (@fst _ _) G))
   (andb (negb (id_in_list id (map (@fst ident Clight.fundef) fs)))
     (semax_body_params_ok f)) = true ->
@@ -290,328 +274,308 @@ Axiom semax_func_cons:
      (fun it : ident * type =>
       complete_type cenv_cs (snd it) =
       true) (fn_vars f) ->
-   var_sizes_ok (f.(fn_vars)) ->
+   var_sizes_ok cenv_cs (f.(fn_vars)) ->
    f.(fn_callconv) = cc ->
    Genv.find_symbol ge id = Some b -> 
    Genv.find_funct_ptr ge b = Some (Internal f) -> 
-  semax_body V G f (id, mk_funspec fsig cc A P Q NEP NEQ) ->
-  semax_func V G ge fs G' ->
-  semax_func V G ge ((id, Internal f)::fs)
-       ((id, mk_funspec fsig cc A P Q NEP NEQ)  :: G').
+  semax_body V G E f (id, mk_funspec fsig cc A P Q) ->
+  semax_func V G ge E fs G' ->
+  semax_func V G ge E ((id, Internal f)::fs)
+       ((id, mk_funspec fsig cc A P Q)  :: G').
 
-Axiom semax_func_cons_ext: forall {Espec:OracleKind} (V: varspecs) (G: funspecs) 
-     {C: compspecs} ge fs id ef argsig retsig A P Q NEP NEQ argsig'
+Axiom semax_func_cons_ext: forall (V: varspecs) (G: funspecs) 
+     {C: compspecs} ge E fs id ef argsig retsig A P Q argsig'
       (G': funspecs) cc b,
   argsig' = typelist2list argsig ->
   ef_sig ef = mksignature (typlist_of_typelist argsig) (rettype_of_type retsig) cc ->
   id_in_list id (map (@fst _ _) fs) = false ->
   (ef_inline ef = false \/ withtype_empty A) ->
-  (forall gx ts x (ret : option val),
-     (Q ts x (make_ext_rval gx (rettype_of_type retsig) ret)
-        && !!Builtins0.val_opt_has_rettype ret (rettype_of_type retsig)
-        |-- !!tc_option_val retsig ret)) ->
+  (forall gx x (ret : option val),
+     (Q x (make_ext_rval gx (rettype_of_type retsig) ret)
+        ∧ ⌜Builtins0.val_opt_has_rettype ret (rettype_of_type retsig)⌝
+        ⊢ ⌜tc_option_val retsig ret⌝)) ->
   Genv.find_symbol ge id = Some b -> Genv.find_funct_ptr ge b = Some (External ef argsig retsig cc) ->
-  @semax_external Espec ef A P Q ->
-  semax_func V G ge fs G' ->
-  semax_func V G ge ((id, External ef argsig retsig cc)::fs)
-       ((id, mk_funspec (argsig', retsig) cc A P Q NEP NEQ)  :: G').
+  (⊢semax_external E ef A P Q) ->
+  semax_func V G ge E fs G' ->
+  semax_func V G ge E ((id, External ef argsig retsig cc)::fs)
+       ((id, mk_funspec (argsig', retsig) cc A P Q)  :: G').
 
-Axiom semax_func_mono: forall  {Espec CS CS'} (CSUB: cspecs_sub CS CS') ge ge'
+Axiom semax_func_mono: forall {CS'} (CSUB: cspecs_sub CS CS') ge ge' E
   (Gfs: forall i,  sub_option (Genv.find_symbol ge i) (Genv.find_symbol ge' i))
   (Gffp: forall b, sub_option (Genv.find_funct_ptr ge b) (Genv.find_funct_ptr ge' b))
-  V G fdecs G1 (H: @semax_func Espec V G CS ge fdecs G1), @semax_func Espec V G CS' ge' fdecs G1.
+  V G fdecs G1 (H: semax_func V G (C := CS) ge E fdecs G1), semax_func V G (C := CS') ge' E fdecs G1.
 
 Axiom semax_func_app:
-  forall Espec ge cs V H funs1 funs2 G1 G2
-         (SF1: @semax_func Espec V H cs ge funs1 G1) (SF2: @semax_func Espec V H cs ge funs2 G2)
+  forall ge E V H funs1 funs2 G1 G2
+         (SF1: semax_func V H ge E funs1 G1) (SF2: semax_func V H ge E funs2 G2)
          (L:length funs1 = length G1),
-    @semax_func Espec V H cs ge (funs1 ++ funs2) (G1++G2).
+    semax_func V H ge E (funs1 ++ funs2) (G1++G2).
   
 Axiom semax_func_subsumption:
-  forall Espec ge cs V V' F F'
-         (SUB: tycontext_sub (nofunc_tycontext V F) (nofunc_tycontext V F'))
-         (HV: forall id, sub_option (make_tycontext_g V F) ! id (make_tycontext_g V' F') ! id),
-  forall funs G (SF: @semax_func Espec V F cs ge funs G),  @semax_func Espec V' F' cs ge funs G.
+  forall ge E V V' F F'
+         (SUB: tycontext_sub E (nofunc_tycontext V F) (nofunc_tycontext V F'))
+         (HV: forall id, sub_option ((make_tycontext_g V F) !! id) ((make_tycontext_g V' F') !! id)),
+  forall funs G (SF: semax_func V F ge E funs G),  semax_func V' F' ge E funs G.
   
 Axiom semax_func_join:
-  forall {Espec cs ge V1 H1 V2 H2 V funs1 funs2 G1 G2 H}
-  (SF1: @semax_func Espec V1 H1 cs ge funs1 G1) (SF2: @semax_func Espec V2 H2 cs ge funs2 G2)
+  forall {ge E V1 H1 V2 H2 V funs1 funs2 G1 G2 H}
+  (SF1: semax_func V1 H1 ge E funs1 G1) (SF2: semax_func V2 H2 ge E funs2 G2)
 
-  (K1: forall i, sub_option ((make_tycontext_g V1 H1) ! i) ((make_tycontext_g V1 H) ! i))
-  (K2: forall i, subsumespec ((make_tycontext_s H1) ! i) ((make_tycontext_s H) ! i))
-  (K3: forall i, sub_option ((make_tycontext_g V1 H) ! i) ((make_tycontext_g V H) ! i))
+  (K1: forall i, sub_option ((make_tycontext_g V1 H1) !! i) ((make_tycontext_g V1 H) !! i))
+  (K2: forall i, subsumespec E ((make_tycontext_s H1) !! i) ((make_tycontext_s H) !! i))
+  (K3: forall i, sub_option ((make_tycontext_g V1 H) !! i) ((make_tycontext_g V H) !! i))
 
-  (N1: forall i, sub_option ((make_tycontext_g V2 H2) ! i) ((make_tycontext_g V2 H) ! i))
-  (N2: forall i, subsumespec ((make_tycontext_s H2) ! i) ((make_tycontext_s H) ! i))
-  (N3: forall i, sub_option ((make_tycontext_g V2 H) ! i) ((make_tycontext_g V H) ! i)),
-  @semax_func Espec V H cs ge (funs1 ++ funs2) (G1++G2).
-  
+  (N1: forall i, sub_option ((make_tycontext_g V2 H2) !! i) ((make_tycontext_g V2 H) !! i))
+  (N2: forall i, subsumespec E ((make_tycontext_s H2) !! i) ((make_tycontext_s H) !! i))
+  (N3: forall i, sub_option ((make_tycontext_g V2 H) !! i) ((make_tycontext_g V H) !! i)),
+semax_func V H ge E (funs1 ++ funs2) (G1++G2).
+
 Axiom semax_func_firstn:
-  forall {Espec cs ge H V n funs G} (SF: @semax_func Espec V H cs ge funs G),
-    @semax_func Espec V H cs ge (firstn n funs) (firstn n G).
-  
-Axiom semax_func_skipn:
-  forall {Espec cs ge H V funs G} (HV:list_norepet (map fst funs))
-         (SF: @semax_func Espec V H cs ge funs G) n,
-    @semax_func Espec V H cs ge (skipn n funs) (skipn n G).
+  forall {ge E H V n funs G} (SF: semax_func V H ge E funs G),
+    semax_func V H ge E (firstn n funs) (firstn n G).
 
-Axiom semax_body_subsumption: forall cs V V' F F' f spec
-      (SF: @semax_body V F cs f spec)
-      (TS: tycontext_sub (func_tycontext f V F nil) (func_tycontext f V' F' nil)),
-  @semax_body V' F' cs f spec.
+Axiom semax_func_skipn:
+  forall {ge E H V funs G} (HV: list_norepet (map fst funs)) (SF: semax_func V H ge E funs G) n,
+    semax_func V H ge E (skipn n funs) (skipn n G).
+
+Axiom semax_body_subsumption: forall V V' F F' E f spec
+      (SF: semax_body V F E f spec)
+      (TS: tycontext_sub E (func_tycontext f V F nil) (func_tycontext f V' F' nil)),
+  semax_body V' F' E f spec.
   
-Axiom semax_body_cenv_sub: forall {CS CS'} (CSUB: cspecs_sub CS CS') V G f spec
+Axiom semax_body_cenv_sub: forall {CS'} (CSUB: cspecs_sub CS CS') V G E f spec
       (COMPLETE : Forall (fun it : ident * type => complete_type (@cenv_cs CS) (snd it) = true) (fn_vars f)),
-  @semax_body V G CS f spec -> @semax_body V G CS' f spec.
+  semax_body V G (C := CS) E f spec -> semax_body V G (C := CS') E f spec.
 
 (* THESE RULES FROM semax_loop *)
 
 Axiom semax_ifthenelse :
-  forall {CS: compspecs} {Espec: OracleKind},
-   forall Delta P (b: expr) c d R,
+   forall E Delta P (b: expr) c d R,
       bool_type (typeof b) = true ->
-     @semax CS Espec Delta (P && local (`(typed_true (typeof b)) (eval_expr b))) c R ->
-     @semax CS Espec Delta (P && local (`(typed_false (typeof b)) (eval_expr b))) d R ->
-     @semax CS Espec Delta (|> (tc_expr Delta (Eunop Cop.Onotbool b (Tint I32 Signed noattr)) && P)) (Sifthenelse b c d) R.
+     semax E Delta (fun rho => P rho ∧ ⌜expr_true b rho⌝) c R ->
+     semax E Delta (fun rho => P rho ∧ ⌜expr_false b rho⌝) d R ->
+     semax E Delta (fun rho => ▷ (tc_expr Delta (Eunop Cop.Onotbool b (Tint I32 Signed noattr)) rho ∧ P rho)) (Sifthenelse b c d) R.
 
 Axiom semax_seq:
-  forall{CS: compspecs} {Espec: OracleKind},
-forall Delta R P Q h t,
-    @semax CS Espec Delta P h (overridePost Q R) ->
-    @semax CS Espec Delta Q t R ->
-    @semax CS Espec Delta P (Ssequence h t) R.
+  forall E Delta (R: ret_assert) P Q h t,
+  semax E Delta P h (overridePost Q R) ->
+  semax E Delta Q t R ->
+  semax E Delta P (Clight.Ssequence h t) R.
 
 Axiom semax_break:
-  forall {CS: compspecs} {Espec: OracleKind},
-   forall Delta Q,    @semax CS Espec Delta (RA_break Q) Sbreak Q.
+   forall E Delta Q,    semax E Delta (RA_break Q) Sbreak Q.
 
 Axiom semax_continue:
-  forall {CS: compspecs} {Espec: OracleKind},
-   forall Delta Q,    @semax CS Espec Delta (RA_continue Q) Scontinue Q.
+   forall E Delta Q,    semax E Delta (RA_continue Q) Scontinue Q.
 
 Axiom semax_loop :
-  forall{CS: compspecs} {Espec: OracleKind},
-forall Delta Q Q' incr body R,
-     @semax CS Espec Delta  Q body (loop1_ret_assert Q' R) ->
-     @semax CS Espec Delta Q' incr (loop2_ret_assert Q R) ->
-     @semax CS Espec Delta Q (Sloop body incr) R.
+forall E Delta Q Q' incr body R,
+     semax E Delta Q body (loop1_ret_assert Q' R) ->
+     semax E Delta Q' incr (loop2_ret_assert Q R) ->
+     semax E Delta Q (Sloop body incr) R.
 
 (* THIS RULE FROM semax_switch *)
 
 Axiom semax_switch: 
-  forall{CS: compspecs} {Espec: OracleKind},
-  forall Delta (Q: environ->mpred) a sl R,
+  forall E Delta (Q: assert) a sl R,
      is_int_type (typeof a) = true ->
-     (forall rho, Q rho |-- tc_expr Delta a rho) ->
+     (forall rho, Q rho ⊢ tc_expr Delta a rho) ->
      (forall n,
-     @semax CS Espec Delta 
-               (local (`eq (eval_expr a) `(Vint n)) &&  Q)
+     semax E Delta 
+               (local (`eq (eval_expr a) `(Vint n)) ∧ Q)
                (seq_of_labeled_statement (select_switch (Int.unsigned n) sl))
                (switch_ret_assert R)) ->
-     @semax CS Espec Delta Q (Sswitch a sl) R.
+     semax E Delta Q (Sswitch a sl) R.
 
 (* THESE RULES FROM semax_call *)
 
-Axiom semax_call: forall {CS Espec},
-  forall Delta (A: rmaps.TypeTree) P Q
-  (NEP: args_super_non_expansive P) (NEQ: super_non_expansive Q)
-  (ts: list Type) x
-   F ret argsig retsig cc a bl,
+Axiom semax_call:
+  forall E Delta (A: Type) P Q x
+   F ret id argsig retsig cc a bl,
            Cop.classify_fun (typeof a) =
            Cop.fun_case_f (typelist_of_type_list argsig) retsig cc ->
             (retsig = Tvoid -> ret = None) ->
           tc_fn_return Delta ret retsig ->
-  @semax CS Espec Delta
-          ((((tc_expr Delta a) && (tc_exprlist Delta argsig bl)))  &&
-         (`(func_ptr (mk_funspec  (argsig,retsig) cc A P Q NEP NEQ)) (eval_expr a) &&
-          (|>(F * (fun rho => P ts x (ge_of rho, eval_exprlist argsig bl rho))))))
+  semax E Delta
+          ((((tc_expr Delta a) ∧ (tc_exprlist Delta argsig bl)))  ∧
+         (assert_of (fun rho => func_ptr (ge_of rho) E id (mk_funspec (argsig,retsig) cc A P Q) (eval_expr a rho)) ∧
+          (▷(F ∗ assert_of (fun rho => P x (ge_of rho, eval_exprlist argsig bl rho))))))
          (Scall ret a bl)
          (normal_ret_assert
-          (EX old:val, substopt ret (`old) F * maybe_retval (Q ts x) retsig ret)).
+          (∃ old:val, assert_of (substopt ret (`old) F) ∗ maybe_retval (Q x) retsig ret)).
 
 Axiom  semax_return :
-  forall {CS: compspecs} {Espec: OracleKind},
-   forall Delta (R: ret_assert) ret ,
-      @semax CS Espec Delta
-                ( (tc_expropt Delta ret (ret_type Delta)) &&
-                `(RA_return R : option val -> environ -> mpred) (cast_expropt ret (ret_type Delta)) (@id environ))
+   forall E Delta (R: ret_assert) ret ,
+      semax E Delta
+                ( (tc_expropt Delta ret (ret_type Delta)) ∧
+                (assert_of (`(RA_return R : option val -> environ -> mpred) (cast_expropt ret (ret_type Delta)) (@id environ))))
                 (Sreturn ret)
                 R.
 
 (* THESE RULES FROM semax_straight *)
 
 Axiom semax_set_forward :
-  forall {CS: compspecs} {Espec: OracleKind},
-forall (Delta: tycontext) (P: environ->mpred) id e,
-    @semax CS Espec Delta
-        (|> ( (tc_expr Delta e) &&
-             (tc_temp_id id (typeof e) Delta e) &&
+forall E (Delta: tycontext) (P: assert) id e,
+    semax E Delta
+        (▷ ( (tc_expr Delta e) ∧
+             (tc_temp_id id (typeof e) Delta e) ∧
           P))
           (Sset id e)
         (normal_ret_assert
-          (EX old:val, local (`eq (eval_id id) (subst id (`old) (eval_expr e))) &&
-                            subst id (`old) P)).
+          (∃ old:val, local (`eq (eval_id id) (subst id (`old) (eval_expr e))) ∧
+                            assert_of (subst id (`old) P))).
 
 Axiom semax_ptr_compare :
-forall{CS: compspecs} {Espec: OracleKind},
-forall (Delta: tycontext) P id cmp e1 e2 ty sh1 sh2,
-    sepalg.nonidentity sh1 -> sepalg.nonidentity sh2 ->
+forall E (Delta: tycontext) P id cmp e1 e2 ty sh1 sh2,
+   sh1 <> Share.bot -> sh2 <> Share.bot ->
    is_comparison cmp = true  ->
    eqb_type (typeof e1) int_or_ptr_type = false ->
    eqb_type (typeof e2) int_or_ptr_type = false ->
    typecheck_tid_ptr_compare Delta id = true ->
-   @semax CS Espec Delta
-        ( |> ( (tc_expr Delta e1) &&
-              (tc_expr Delta e2)  &&
+   semax E Delta
+        ( ▷ ( (tc_expr Delta e1) ∧
+              (tc_expr Delta e2)  ∧
 
-          local (`(blocks_match cmp) (eval_expr e1) (eval_expr e2)) &&
-          (`(mapsto_ sh1 (typeof e1)) (eval_expr e1) * TT) &&
-          (`(mapsto_ sh2 (typeof e2)) (eval_expr e2) * TT) &&
+          local (`(blocks_match cmp) (eval_expr e1) (eval_expr e2)) ∧
+          <absorb> assert_of (`(mapsto_ sh1 (typeof e1)) (eval_expr e1)) ∧
+          <absorb> assert_of (`(mapsto_ sh2 (typeof e2)) (eval_expr e2)) ∧
           P))
           (Sset id (Ebinop cmp e1 e2 ty))
         (normal_ret_assert
-          (EX old:val,
+          (∃ old:val,
                  local (`eq (eval_id id)  (subst id `(old)
-                     (eval_expr (Ebinop cmp e1 e2 ty)))) &&
-                            subst id `(old) P)).
+                     (eval_expr (Ebinop cmp e1 e2 ty)))) ∧
+                            assert_of (subst id `(old) P))).
 
 Axiom semax_load :
-  forall {CS: compspecs} {Espec: OracleKind},
-forall (Delta: tycontext) sh id P e1 t2 (v2: val),
+forall E (Delta: tycontext) sh id P e1 t2 (v2: val),
     typeof_temp Delta id = Some t2 ->
     is_neutral_cast (typeof e1) t2 = true ->
     readable_share sh ->
-    (local (tc_environ Delta) && P |-- `(mapsto sh (typeof e1)) (eval_lvalue e1) (`v2) * TT) ->
-    @semax CS Espec Delta
-       (|> ( (tc_lvalue Delta e1) &&
-       local (`(tc_val (typeof e1) v2)) &&
+    (local (tc_environ Delta) ∧ P ⊢ <absorb> assert_of (`(mapsto sh (typeof e1)) (eval_lvalue e1) (`v2))) ->
+    semax E Delta
+       (▷ ( (tc_lvalue Delta e1) ∧
+       local (`(tc_val (typeof e1) v2)) ∧
           P))
        (Sset id e1)
-       (normal_ret_assert (EX old:val, local (`eq (eval_id id) (`v2)) &&
-                                          (subst id (`old) P))).
+       (normal_ret_assert (∃ old:val, local (`eq (eval_id id) (`v2)) ∧
+                                          assert_of (subst id (`old) P))).
 
 Axiom semax_cast_load :
-  forall {CS: compspecs} {Espec: OracleKind},
-forall (Delta: tycontext) sh id P e1 t1 (v2: val),
+forall E (Delta: tycontext) sh id P e1 t1 (v2: val),
     typeof_temp Delta id = Some t1 ->
    cast_pointer_to_bool (typeof e1) t1 = false ->
     readable_share sh ->
-    (local (tc_environ Delta) && P |-- `(mapsto sh (typeof e1)) (eval_lvalue e1) (`v2) * TT) ->
-    @semax CS Espec Delta
-       (|> ( (tc_lvalue Delta e1) &&
-       local (`(tc_val t1) (`(eval_cast (typeof e1) t1 v2))) &&
+    (local (tc_environ Delta) ∧ P ⊢ <absorb> assert_of (`(mapsto sh (typeof e1)) (eval_lvalue e1) (`v2))) ->
+    semax E Delta
+       (▷ ( (tc_lvalue Delta e1) ∧
+       local (`(tc_val t1) (`(eval_cast (typeof e1) t1 v2))) ∧
           P))
        (Sset id (Ecast e1 t1))
-       (normal_ret_assert (EX old:val, local (`eq (eval_id id) (`(eval_cast (typeof e1) t1 v2))) &&
-                                          (subst id (`old) P))).
+       (normal_ret_assert (∃ old:val, local (`eq (eval_id id) (`(eval_cast (typeof e1) t1 v2))) ∧
+                                          assert_of (subst id (`old) P))).
 
 Axiom semax_store:
-  forall {CS: compspecs} {Espec: OracleKind},
- forall Delta e1 e2 sh P,
+ forall E Delta e1 e2 sh P,
    writable_share sh ->
-   @semax CS Espec Delta
-          (|> ( (tc_lvalue Delta e1) &&  (tc_expr Delta (Ecast e2 (typeof e1)))  &&
-             (`(mapsto_ sh (typeof e1)) (eval_lvalue e1) * P)))
+   semax E Delta
+          (▷ ( (tc_lvalue Delta e1) ∧  (tc_expr Delta (Ecast e2 (typeof e1)))  ∧
+             (assert_of (`(mapsto_ sh (typeof e1)) (eval_lvalue e1)) ∗ P)))
           (Sassign e1 e2)
           (normal_ret_assert
-               (`(mapsto sh (typeof e1)) (eval_lvalue e1) (`force_val (`(sem_cast (typeof e2) (typeof e1)) (eval_expr e2))) * P)).
+               (assert_of (`(mapsto sh (typeof e1)) (eval_lvalue e1) (`force_val (`(sem_cast (typeof e2) (typeof e1)) (eval_expr e2)))) ∗ P)).
 
 Axiom semax_store_union_hack:
-     forall {cs: compspecs} {Espec:OracleKind}
-          (Delta : tycontext) (e1 e2 : expr) (t2: type) (ch ch' : memory_chunk) (sh : share) (P : LiftEnviron mpred),
+     forall E (Delta : tycontext) (e1 e2 : expr) (t2: type) (ch ch' : memory_chunk) (sh : share) (P : assert),
        (numeric_type (typeof e1) && numeric_type t2)%bool = true ->
        access_mode (typeof e1) = By_value ch ->
        access_mode t2 = By_value ch' ->
        decode_encode_val_ok ch ch' ->
        writable_share sh ->
-       semax Delta
-         (|> (tc_lvalue Delta e1 && tc_expr Delta (Ecast e2 (typeof e1)) &&
-              ((`(mapsto_ sh (typeof e1)) (eval_lvalue e1) 
-                && `(mapsto_ sh t2) (eval_lvalue e1))
-               * P)))
+       semax E Delta
+         (▷ (tc_lvalue Delta e1 ∧ tc_expr Delta (Ecast e2 (typeof e1)) ∧
+              ((assert_of (`(mapsto_ sh (typeof e1)) (eval_lvalue e1))
+                ∧ assert_of (`(mapsto_ sh t2) (eval_lvalue e1)))
+               ∗ P)))
          (Sassign e1 e2)
          (normal_ret_assert
-            (EX v':val, 
-              andp (local  ((`decode_encode_val )
-                         ((` force_val) ((`(sem_cast (typeof e2) (typeof e1))) (eval_expr e2))) (`ch) (`ch') (`v') ))
-              ((` (mapsto sh t2)) (eval_lvalue e1) (`v') * P))).
+            (∃ v':val,
+              (local  ((`decode_encode_val )
+                         ((` force_val) ((`(sem_cast (typeof e2) (typeof e1))) (eval_expr e2))) (`ch) (`ch') (`v') )) ∧
+              (assert_of ((` (mapsto sh t2)) (eval_lvalue e1) (`v')) ∗ P))).
 
 (* THESE RULES FROM semax_lemmas *)
 
 Axiom semax_skip:
-  forall {CS: compspecs} {Espec: OracleKind},
-   forall Delta P, @semax CS Espec Delta P Sskip (normal_ret_assert P).
+   forall E Delta P, semax E Delta P Sskip (normal_ret_assert P).
 
 Axiom semax_conseq:
-  forall {CS: compspecs} {Espec: OracleKind},
-  forall Delta (P' : environ -> mpred) (R': ret_assert) P c (R: ret_assert) ,
-    (local (tc_environ Delta) && ((allp_fun_id Delta) && P) |-- (|={Ensembles.Full_set}=> P')) ->
-    (local (tc_environ Delta) && ((allp_fun_id Delta) && RA_normal R') |-- (|={Ensembles.Full_set}=> RA_normal R)) ->
-    (local (tc_environ Delta) && ((allp_fun_id Delta) && RA_break R') |-- (|={Ensembles.Full_set}=> RA_break R)) ->
-    (local (tc_environ Delta) && ((allp_fun_id Delta) && RA_continue R') |-- (|={Ensembles.Full_set}=> RA_continue R)) ->
-    (forall vl, local (tc_environ Delta) && ((allp_fun_id Delta) && RA_return R' vl) |-- (RA_return R vl)) ->
-   @semax CS Espec Delta P' c R' -> @semax CS Espec Delta P c R.
+  forall E Delta (P' : assert) (R': ret_assert) P c (R: ret_assert),
+    (local (tc_environ Delta) ∧ ((allp_fun_id E Delta) ∧ P) ⊢ (|={E}=> P')) ->
+    (local (tc_environ Delta) ∧ ((allp_fun_id E Delta) ∧ RA_normal R') ⊢ (|={E}=> RA_normal R)) ->
+    (local (tc_environ Delta) ∧ ((allp_fun_id E Delta) ∧ RA_break R') ⊢ (|={E}=> RA_break R)) ->
+    (local (tc_environ Delta) ∧ ((allp_fun_id E Delta) ∧ RA_continue R') ⊢ (|={E}=> RA_continue R)) ->
+    (forall vl, local (tc_environ Delta) ∧ ((allp_fun_id E Delta) ∧ RA_return R' vl) ⊢ (RA_return R vl)) ->
+   semax E Delta P' c R' -> semax E Delta P c R.
 
 Axiom semax_Slabel:
-   forall {cs:compspecs} {Espec: OracleKind},
      forall Delta (P:environ -> mpred) (c:statement) (Q:ret_assert) l,
-   @semax cs Espec Delta P c Q -> @semax cs Espec Delta P (Slabel l c) Q.
+   semax E Delta P c Q -> semax E Delta P (Slabel l c) Q.
 
 (* THESE RULES FROM semax_ext *)
 
 (*TODO: What's the preferred way to expose these defs in the SL interface?*)
 Axiom semax_ext:
-  forall  (Espec : OracleKind)
-         (ext_link: Strings.String.string -> ident)
+  forall E (ext_link: Strings.String.string -> ident)
          (id : Strings.String.string) (sig : compcert_rmaps.typesig) (sig' : signature)
-         cc A P Q NEP NEQ (fs : funspecs),
-  let f := mk_funspec sig cc A P Q NEP NEQ in
+         cc A P Q (fs : funspecs),
+  let f := mk_funspec sig cc A P Q in
   In (ext_link id,f) fs ->
   funspecs_norepeat fs ->
   sig' = semax_ext.typesig2signature sig cc ->
-  @semax_external (add_funspecs Espec ext_link fs) (EF_external id sig') _ P Q.
+  ⊢ semax_external {| OK_ty := OK_ty; OK_spec := add_funspecs_rec OK_ty ext_link OK_spec fs |} (EF_external id sig') _ P Q.
 
 Axiom semax_external_FF:
- forall Espec ef A,
-  @semax_external Espec ef A (fun _ _ => FF) (fun _ _ => FF).
+ forall ef A,
+  semax_external ef A (fun _ _ => False) (fun _ _ => False).
 
-Axiom semax_external_binaryintersection: 
+(*Axiom semax_external_binaryintersection: 
 forall {Espec ef A1 P1 Q1 P1ne Q1ne A2 P2 Q2 P2ne Q2ne 
       A P Q P_ne Q_ne sig cc}
-  (EXT1: @semax_external Espec ef A1 P1 Q1)
-  (EXT2: @semax_external Espec ef A2 P2 Q2)
+  (∃T1: @semax_external Espec ef A1 P1 Q1)
+  (∃T2: @semax_external Espec ef A2 P2 Q2)
   (BI: binary_intersection (mk_funspec sig cc A1 P1 Q1 P1ne Q1ne) 
                       (mk_funspec sig cc A2 P2 Q2 P2ne Q2ne) =
      Some (mk_funspec sig cc A P Q P_ne Q_ne))
   (LENef: length (fst sig) = length (sig_args (ef_sig ef))),
-  @semax_external Espec ef A P Q.
+  @semax_external Espec ef A P Q.*)
 
 Axiom semax_external_funspec_sub: forall 
-  (DISABLE: False) {Espec argtypes rtype cc ef A1 P1 Q1 P1ne Q1ne A P Q Pne Qne}
+  {E argtypes rtype cc ef A1 P1 Q1 A P Q}
   (Hsub: funspec_sub (mk_funspec (argtypes, rtype) cc A1 P1 Q1 P1ne Q1ne) 
                    (mk_funspec (argtypes, rtype) cc A P Q Pne Qne))
   (HSIG: ef_sig ef = 
          mksignature (map typ_of_type argtypes)
-                     (rettype_of_type rtype) cc)
-  (SE: @semax_external Espec ef A1 P1 Q1),
-  @semax_external Espec ef A P Q.
+                     (rettype_of_type rtype) cc),
+  semax_external E ef A1 P1 Q1 ⊢ semax_external E ef A P Q.
 
-Axiom semax_body_binaryintersection:
+(*Axiom semax_body_binaryintersection:
 forall {V G cs} f sp1 sp2 phi
   (SB1: @semax_body V G cs f sp1) (SB2: @semax_body V G cs f sp2)
   (BI: binary_intersection (snd sp1) (snd sp2) = Some phi),
-  @semax_body V G cs f (fst sp1, phi).
+  @semax_body V G cs f (fst sp1, phi).*)
 
-Axiom semax_body_funspec_sub: forall {V G cs f i phi phi'} 
-  (SB: @semax_body V G cs f (i, phi)) (Sub: funspec_sub phi phi')
+Axiom semax_body_funspec_sub: forall {V G E f i phi phi'} 
+  (SB: semax_body V G E f (i, phi)) (Sub: funspec_sub E phi phi')
   (LNR: list_norepet (map fst (fn_params f) ++ map fst (fn_temps f))),
-  @semax_body V G cs f (i, phi').
+  semax_body V G E f (i, phi').
 
 Axiom semax_Delta_subsumption:
-  forall {CS: compspecs} {Espec: OracleKind},
-  forall Delta Delta' P c R,
-       tycontext_sub Delta Delta' ->
-       @semax CS Espec Delta P c R -> @semax CS Espec Delta' P c R.
+  forall E Delta Delta' P c R,
+       tycontext_sub E Delta Delta' ->
+       semax E Delta P c R -> semax E Delta' P c R.
+
+End mpred.
 
 End MINIMUM_CLIGHT_SEPARATION_HOARE_LOGIC.
 
@@ -622,124 +586,120 @@ Declare Module CSHL_MinimumLogic: MINIMUM_CLIGHT_SEPARATION_HOARE_LOGIC.
 Import CSHL_MinimumLogic.CSHL_Def.
 Import CSHL_MinimumLogic.CSHL_Defs.
 
+Section mpred.
+
+Context `{!heapGS Σ} {Espec: OracleKind} `{!externalGS (OK_ty(Σ := Σ)) Σ} {CS: compspecs}.
+
 Axiom semax_set :
-  forall {CS: compspecs} {Espec: OracleKind},
-forall (Delta: tycontext) (P: environ->mpred) id e,
-    @semax CS Espec Delta
-        (|> ( (tc_expr Delta e) &&
-             (tc_temp_id id (typeof e) Delta e) &&
+forall E (Delta: tycontext) (P: environ->mpred) id e,
+    semax E Delta
+        (▷ ( (tc_expr Delta e) ∧
+             (tc_temp_id id (typeof e) Delta e) ∧
              subst id (eval_expr e) P))
           (Sset id e) (normal_ret_assert P).
 
 Axiom semax_fun_id:
-  forall {CS: compspecs} {Espec: OracleKind},
-      forall id f Delta P Q c,
-    (var_types Delta) ! id = None ->
-    (glob_specs Delta) ! id = Some f ->
-    (glob_types Delta) ! id = Some (type_of_funspec f) ->
-    @semax CS Espec Delta (P && `(func_ptr f) (eval_var id (type_of_funspec f)))
+      forall id f E Delta P Q c,
+    (var_types Delta) !! id = None ->
+    (glob_specs Delta) !! id = Some f ->
+    (glob_types Delta) !! id = Some (type_of_funspec f) ->
+    semax E Delta (P ∧ `(func_ptr f) (eval_var id (type_of_funspec f)))
                   c Q ->
-    @semax CS Espec Delta P c Q.
+    semax E Delta P c Q.
 
-Axiom semax_unfold_Ssequence: forall {CS: compspecs} {Espec: OracleKind} c1 c2,
+Axiom semax_unfold_Ssequence: forall c1 c2,
   unfold_Ssequence c1 = unfold_Ssequence c2 ->
-  (forall P Q Delta, @semax CS Espec Delta P c1 Q -> @semax CS Espec Delta P c2 Q).
+  (forall P Q E Delta, semax E Delta P c1 Q -> semax E Delta P c2 Q).
 
 Axiom seq_assoc:
-  forall {CS: compspecs} {Espec: OracleKind},
-   forall Delta P s1 s2 s3 R,
-        @semax CS Espec Delta P (Ssequence s1 (Ssequence s2 s3)) R <->
-        @semax CS Espec Delta P (Ssequence (Ssequence s1 s2) s3) R.
+   forall E Delta P s1 s2 s3 R,
+        semax E Delta P (Ssequence s1 (Ssequence s2 s3)) R <->
+        semax E Delta P (Ssequence (Ssequence s1 s2) s3) R.
 
 Axiom semax_seq_skip:
-  forall {CS: compspecs} {Espec: OracleKind},
-  forall Delta P s Q,
-    @semax CS Espec Delta P s Q <-> @semax CS Espec Delta P (Ssequence s Sskip) Q.
+  forall E Delta P s Q,
+    semax E Delta P s Q <-> semax E Delta P (Ssequence s Sskip) Q.
 
 Axiom semax_skip_seq:
-  forall {CS: compspecs} {Espec: OracleKind},
-  forall Delta P s Q,
-    @semax CS Espec Delta P s Q <-> @semax CS Espec Delta P (Ssequence Sskip s) Q.
+  forall E Delta P s Q,
+    semax E Delta P s Q <-> semax E Delta P (Ssequence Sskip s) Q.
 
 Axiom semax_loop_nocontinue1:
-  forall CS Espec Delta Pre s1 s2 s3 Post,
+  forall E Delta Pre s1 s2 s3 Post,
   nocontinue s1 = true ->
   nocontinue s2 = true ->
   nocontinue s3 = true ->
-   @semax CS Espec Delta Pre (Sloop (Ssequence s1 (Ssequence s2 s3)) Sskip) Post ->
-    @semax CS Espec Delta Pre (Sloop (Ssequence s1 s2) s3) Post.
+   semax E Delta Pre (Sloop (Ssequence s1 (Ssequence s2 s3)) Sskip) Post ->
+    semax E Delta Pre (Sloop (Ssequence s1 s2) s3) Post.
 
 Axiom semax_loop_nocontinue:
-  forall {CS: compspecs} {Espec: OracleKind},
- forall Delta P body incr R,
- @semax CS Espec Delta P (Ssequence body incr) (loop_nocontinue_ret_assert P R) ->
- @semax CS Espec Delta P (Sloop body incr) R.
+ forall E Delta P body incr R,
+ semax E Delta P (Ssequence body incr) (loop_nocontinue_ret_assert P R) ->
+ semax E Delta P (Sloop body incr) R.
 
 Axiom semax_convert_for_while':
- forall CS Espec Delta Pre s1 e2 s3 s4 s5 Post,
+ forall E Delta Pre s1 e2 s3 s4 s5 Post,
   nocontinue s4 = true ->
   nocontinue s3 = true -> 
-  @semax CS Espec Delta Pre 
+  semax E Delta Pre 
     (Ssequence s1 (Ssequence (Swhile e2 (Ssequence s4 s3)) s5)) Post ->
-  @semax CS Espec Delta Pre (Ssequence (Sfor s1 e2 s4 s3) s5) Post.
+  semax E Delta Pre (Ssequence (Sfor s1 e2 s4 s3) s5) Post.
 
 Axiom semax_loop_unroll1:
-  forall {CS: compspecs} {Espec: OracleKind} Delta P P' Q body incr R,
-  @semax CS Espec Delta P body (loop1_ret_assert P' R) ->
-  @semax CS Espec Delta P' incr (loop2_ret_assert Q R) ->
-  @semax CS Espec Delta Q (Sloop body incr) R ->
-  @semax CS Espec Delta P (Sloop body incr) R.
+  forall E Delta P P' Q body incr R,
+  semax E Delta P body (loop1_ret_assert P' R) ->
+  semax E Delta P' incr (loop2_ret_assert Q R) ->
+  semax E Delta Q (Sloop body incr) R ->
+  semax E Delta P (Sloop body incr) R.
 
 Axiom semax_if_seq:
- forall {CS: compspecs} {Espec: OracleKind} Delta P e c1 c2 c Q,
+ forall E Delta P e c1 c2 c Q,
  semax Delta P (Sifthenelse e (Ssequence c1 c) (Ssequence c2 c)) Q ->
  semax Delta P (Ssequence (Sifthenelse e c1 c2) c) Q.
 
 Axiom semax_seq_Slabel:
-   forall {cs:compspecs} {Espec: OracleKind},
-     forall Delta (P:environ -> mpred) (c1 c2:statement) (Q:ret_assert) l,
-   @semax cs Espec Delta P (Ssequence (Slabel l c1) c2) Q <-> 
-   @semax cs Espec Delta P (Slabel l (Ssequence c1 c2)) Q.
+     forall E Delta (P:environ -> mpred) (c1 c2:statement) (Q:ret_assert) l,
+   semax E Delta P (Ssequence (Slabel l c1) c2) Q <-> 
+   semax E Delta P (Slabel l (Ssequence c1 c2)) Q.
 
 (**************** END OF stuff from semax_rules ***********)
 
 Axiom semax_frame:
-  forall {CS: compspecs} {Espec: OracleKind},
-  forall Delta P s R F,
+  forall E Delta P s R F,
    closed_wrt_modvars s F ->
-  @semax CS Espec Delta P s R ->
-    @semax CS Espec Delta (P * F) s (frame_ret_assert R F).
+  semax E Delta P s R ->
+    semax E Delta (P * F) s (frame_ret_assert R F).
 
 Axiom semax_extract_prop:
-  forall {CS: compspecs} {Espec: OracleKind},
-  forall Delta (PP: Prop) P c Q,
-           (PP -> @semax CS Espec Delta P c Q) ->
-           @semax CS Espec Delta (!!PP && P) c Q.
+  forall E Delta (PP: Prop) P c Q,
+           (PP -> semax E Delta P c Q) ->
+           semax E Delta (⌜PP⌝ ∧ P) c Q.
 
 Axiom semax_extract_later_prop:
-  forall {CS: compspecs} {Espec: OracleKind},
-  forall Delta (PP: Prop) P c Q,
-           (PP -> @semax CS Espec Delta P c Q) ->
-           @semax CS Espec Delta ((|> !!PP) && P) c Q.
+  forall E Delta (PP: Prop) P c Q,
+           (PP -> semax E Delta P c Q) ->
+           semax E Delta ((▷ ⌜PP⌝) ∧ P) c Q.
 
-Axiom semax_adapt_frame: forall {cs Espec} Delta c (P P': assert) (Q Q' : ret_assert)
-   (H: forall rho,  derives (!!(typecheck_environ Delta rho) && (allp_fun_id Delta rho && P rho))
-                   (EX F: assert, (!!(closed_wrt_modvars c F) && (|={Ensembles.Full_set}=> P' rho * F rho) &&
-                         !!(forall rho, (local (tc_environ Delta) rho) && ((allp_fun_id Delta rho)) && RA_normal (frame_ret_assert Q' F) rho |-- (|={Ensembles.Full_set}=> RA_normal Q rho)) &&
-                         !!(forall rho, (local (tc_environ Delta) rho) && ((allp_fun_id Delta rho)) && RA_break (frame_ret_assert Q' F) rho |-- (|={Ensembles.Full_set}=> RA_break Q rho)) &&
-                         !!(forall rho, (local (tc_environ Delta) rho) && ((allp_fun_id Delta rho)) && RA_continue (frame_ret_assert Q' F) rho |-- (|={Ensembles.Full_set}=> RA_continue Q rho)) &&
-                         !!(forall vl rho, (local (tc_environ Delta) rho) && ((allp_fun_id Delta rho)) && RA_return (frame_ret_assert Q' F) vl rho |-- (RA_return Q vl rho)))))
-   (SEM: @semax cs Espec Delta P' c Q'),
-   @semax cs Espec Delta P c Q.
+Axiom semax_adapt_frame: forall E Delta c (P P': assert) (Q Q' : ret_assert)
+   (H: forall rho, ⌜typecheck_environ Delta rho⌝ ∧ (<affine> allp_fun_id E Delta rho ∗ P rho) ⊢
+                   ∃ F: assert, (⌜closed_wrt_modvars c F⌝ ∧ |={E}=> (P' rho ∗ F rho) ∧
+                         ⌜forall rho, ((local (tc_environ Delta) rho) ∧ <affine> allp_fun_id E Delta rho ∗ RA_normal (frame_ret_assert Q' F) rho ⊢ |={E}=> RA_normal Q rho)⌝ ∧
+                         ⌜forall rho, ((local (tc_environ Delta) rho) ∧ <affine> allp_fun_id E Delta rho ∗ RA_break (frame_ret_assert Q' F) rho ⊢ |={E}=> RA_break Q rho)⌝ ∧
+                         ⌜forall rho, ((local (tc_environ Delta) rho) ∧ <affine> allp_fun_id E Delta rho ∗ RA_continue (frame_ret_assert Q' F) rho ⊢ |={E}=> RA_continue Q rho)⌝ ∧
+                         ⌜forall vl rho, ((local (tc_environ Delta) rho) ∧ <affine> allp_fun_id E Delta rho ∗ RA_return (frame_ret_assert Q' F) vl rho ⊢ RA_return Q vl rho)⌝))
+   (SEM: semax E Delta P' c Q'),
+   semax E Delta P c Q.
 
-Axiom semax_adapt: forall {cs Espec} Delta c (P P': assert) (Q Q' : ret_assert)
-   (H: forall rho,  !!(typecheck_environ Delta rho) && (allp_fun_id Delta rho && P rho)
-                   |-- ((|={Ensembles.Full_set}=> P' rho) &&
-                        !!(forall rho, RA_normal Q' rho |-- (|={Ensembles.Full_set}=> RA_normal Q rho)) &&
-                        !!(forall rho, RA_break Q' rho |-- (|={Ensembles.Full_set}=> RA_break Q rho)) &&
-                        !!(forall rho, RA_continue Q' rho |-- (|={Ensembles.Full_set}=> RA_continue Q rho)) &&
-                        !!(forall vl rho, RA_return Q' vl rho |-- (RA_return Q vl rho))))
-   (SEM: @semax cs Espec Delta P' c Q'),
-   @semax cs Espec Delta P c Q.
+Axiom semax_adapt: forall E Delta c (P P': assert) (Q Q' : ret_assert)
+   (H: forall rho,  ⌜typecheck_environ Delta rho⌝ ∧ (<affine> allp_fun_id E Delta rho ∗ P rho) ⊢
+                   (|={E}=> (P' rho) ∧
+                        ⌜forall rho, RA_normal Q' rho ⊢ |={E}=> RA_normal Q rho⌝ ∧
+                        ⌜forall rho, RA_break Q' rho ⊢ |={E}=> RA_break Q rho⌝ ∧
+                        ⌜forall rho, RA_continue Q' rho ⊢ |={E}=> RA_continue Q rho⌝ ∧
+                        ⌜forall vl rho, RA_return Q' vl rho ⊢ RA_return Q vl rho⌝))
+   (SEM: semax E Delta P' c Q'),
+   semax E Delta P c Q.
+
+End mpred.
 
 End PRACTICAL_CLIGHT_SEPARATION_HOARE_LOGIC.
