veric/semax_loop.v
@@ -76,7 +76,7 @@ Proof.
   assert (cenv_sub (@cenv_cs CS) psi) by (eapply cenv_sub_trans; destruct HGG; auto).
   iCombine "Hm P" as "H"; rewrite (add_and (_ ∗ _) (▷_)); last by iIntros "H"; iNext; iDestruct "H" as "(Hm & H & _)"; iApply (eval_expr_relate(CS := CS) with "[$Hm $H]").
   iDestruct "H" as "(H & >%Heval)".
-  rewrite /tc_expr /typecheck_expr denote_tc_assert_andp; fold (typecheck_expr(CS := CS)).
+  rewrite /tc_expr /typecheck_expr /= denote_tc_assert_andp; fold (typecheck_expr(CS := CS)).
   rewrite -assoc (bi.and_elim_r (denote_tc_assert _ _)).
   rewrite (add_and (_ ∗ _) (▷_)); last by iIntros "H"; iNext; iDestruct "H" as "(Hm & H & _)"; iApply (eval_expr_relate(CS := CS) with "[$Hm $H]").
   iDestruct "H" as "(H & >%Hb)".
